Array bin search (work in progress).

code/dafny/array_search.dfy
@@ -1,3 +1,4 @@
+// Sequential search
 method has_sequential(a: array<int>, key: int) returns (ret: int)
     requires a != null
     requires a.Length > 0
@@ -18,5 +19,44 @@ method has_sequential(a: array<int>, key: int) returns (ret: int)
         }
     }
 
+function sorted(a: array<int>, index: int): bool
+    requires a != null;
+    requires a.Length > 0;
+    requires index >= 0;
+    requires index < a.Length;
+    decreases a.Length - index;
+    { 
+        if (index == a.Length - 1) then true 
+        else if (index < a.Length - 1) then sorted(a, index + 1) 
+        else false 
+    }
 
-//has binary
+// Binary search
+method has_binary(a: array<int>, key: int) returns (ret: int)
+    requires a != null;
+    requires a.Length > 0;
+    requires sorted(a, 0);
+    // result = 0 => key belongs elements(a)
+    {
+        var min, max, x: int;
+        //Init
+        min := 0;
+        max := a.Length - 1;
+        x := 0;
+        while(max != min)
+        invariant min >= 0;
+        invariant max < a.Length;
+        invariant min <= x;
+        invariant max >= x;
+        //Add invariantL Key belongs to a elements
+        //decreases max - min;
+        {
+            x := (max + min) / 2;
+            if a[x] < key {
+                min := x + 1;
+            } else {
+                max := x;
+            }
+            ret := min;
+        }
+    }
